WIP

src/CertifyFacts.v
@@ -43,40 +43,165 @@ Proof.
   - inv H; inv STEP; ss.
 Qed.
 
-Lemma rtc_state_step_certify_bot
-      m1 m2 tid st lc
-      (STEPS: rtc (Machine.step ExecUnit.state_step) m1 m2)
-      (WF: Machine.wf m1)
-      (NOPROMISE: Machine.no_promise m2)
-      (FIND: IdMap.find tid m1.(Machine.tpool) = Some (st, lc)):
-  certify tid (ExecUnit.mk st lc m1.(Machine.mem)) Lock.init.
+Inductive void_taint (v:Taint.t): Prop :=
+| void_taint_intro
+    (TAINT: forall from to loc, ~ v (Taint.W from to loc))
+.
+
+Inductive void_view (v:View.t (A:=Taint.t)): Prop :=
+| void_view_intro
+    (VIEW: void_taint v.(View.annot))
+.
+
+Inductive void_val (v:ValA.t (A:=View.t (A:=Taint.t))): Prop :=
+| void_val_intro
+    (VAL: void_view v.(ValA.annot))
+.
+
+Inductive void_rmap (rmap:RMap.t (A:=View.t (A:=Taint.t))): Prop :=
+| void_rmap_intro
+    (RMAP: IdMap.Forall (fun _ => void_val) rmap)
+.
+
+Inductive void_lc (tid:Id.t) (lc:Local.t (A:=Taint.t)) (mem:Memory.t): Prop :=
+| void_lc_intro
+    (VRP: void_view lc.(Local.vrp))
+    (VWP: void_view lc.(Local.vwp))
+    (VRM: void_view lc.(Local.vrm))
+    (VWM: void_view lc.(Local.vwm))
+    (VCAP: void_view lc.(Local.vcap))
+    (VREL: void_view lc.(Local.vrel))
+    (FWDBANK: forall l fwd (FWD: lc.(Local.fwdbank) l = Some fwd), void_view fwd.(FwdItem.view))
+.
+
+Inductive void_aeu (tid:Id.t) (aeu:AExecUnit.t): Prop :=
+| void_aeu_intro
+    (ST: void_rmap aeu.(ExecUnit.state).(State.rmap))
+    (LC: void_lc tid aeu.(ExecUnit.local) aeu.(ExecUnit.mem))
+    (TAINT: void_taint aeu.(AExecUnit.aux).(AExecUnit.taint))
+    (RELEASE: aeu.(AExecUnit.aux).(AExecUnit.release) = bot)
+.
+
+Lemma void_taint_join
+      l r
+      (L: void_taint l)
+      (R: void_taint r):
+  void_taint (join l r).
 Proof.
-  revert tid st lc FIND NOPROMISE. induction STEPS.
-  { econs; eauto; ss.
-    - eapply NOPROMISE. eauto.
-    - funext. unfold bot, fun_bot. i. propext. econs; ss. i. inv H; ss.
-  }
-  i. inv H. exploit IHSTEPS; ss.
-  { eapply Machine.step_state_step_wf; eauto. }
-  { rewrite TPOOL, IdMap.add_spec, FIND.
-    instantiate (1 := if equiv_dec tid tid0 then lc2 else lc).
-    instantiate (1 := if equiv_dec tid tid0 then st2 else st).
-    condtac; ss.
-  }
-  condtac.
-  - inversion e. subst. rewrite FIND in FIND0. inv FIND0.
-    admit. (* certify is preserved if I executed a state_step. *)
-  - admit. (* certify is preserved if another thread is executed. *)
+  inv L. inv R. econs. ii. inv H.
+  - eapply TAINT. eauto.
+  - eapply TAINT0. eauto.
+Qed.
+
+Lemma void_taint_bot:
+  void_taint bot.
+Proof.
+  econs. ss.
+Qed.
+
+Lemma void_view_join
+      v1 v2
+      (V1: void_view v1)
+      (V2: void_view v2):
+  void_view (join v1 v2).
+Proof.
+  inv V1. inv V2. econs. eapply void_taint_join; eauto.
+Qed.
+
+Lemma void_view_bot:
+  void_view bot.
+Proof.
+  econs. apply void_taint_bot.
+Qed.
+
+Lemma void_rmap_expr
+      rmap e
+      (RMAP: void_rmap rmap):
+  void_view (sem_expr rmap e).(ValA.annot).
+Proof.
+  induction e; ss.
+  - apply void_view_bot.
+  - unfold RMap.find. destruct (IdMap.find reg rmap) eqn:V.
+    + eapply RMAP. eauto.
+    + apply void_view_bot.
+  - apply void_view_join; ss.
+Qed.
+
+Lemma void_rmap_add
+      l v rmap
+      (RMAP: void_rmap rmap)
+      (V: void_val v):
+  void_rmap (RMap.add l v rmap).
+Proof.
+  inv RMAP. econs. ii. revert FIND.
+  unfold RMap.add. rewrite IdMap.add_spec. condtac.
+  - inversion e. i. inv FIND. ss.
+  - apply RMAP0.
+Qed.
+
+Lemma void_aeu_step
+      tid aeu1 aeu2
+      (STEP: AExecUnit.state_step tid aeu1 aeu2)
+      (SOUND: void_aeu tid aeu1):
+  void_aeu tid aeu2.
+Proof.
+  destruct aeu1 as [[st1 lc1 mem1] aux1].
+  destruct aeu2 as [[st2 lc2 mem2] aux2].
+  inv STEP. inv STEP0. inv SOUND. ss. subst.
+  inv LOCAL; ss; inv STATE; ss.
+  - econs; ss.
+    inv LC0. inv LC. econs; eauto using void_view_join, void_view_bot, void_rmap_expr.
+  - econs; ss.
+    + apply void_rmap_add; ss. econs. apply void_rmap_expr. ss.
+    + inv LC0. inv LC. econs; eauto using void_view_join, void_view_bot, void_rmap_expr.
+  - econs; ss.
+    inv LC0. inv LC. econs; eauto using void_view_join, void_view_bot, void_rmap_expr.
+  - econs; ss.
+    inv LC0. inv LC. econs; eauto using void_view_join, void_view_bot, void_rmap_expr.
+  - inv STEP. ss. econs; ss.
+    + apply void_rmap_add; ss. econs. econs. s.
+      admit.
+    + inv LC. econs; s; eauto using void_view_join, void_view_bot, void_rmap_expr.
+      all: admit.
+    + destruct ex; ss.
+    + destruct ex; ss.
+  - inv STEP. ss. econs; ss.
+    + apply void_rmap_add; ss. econs. admit. (* view_ext *)
+    + inv LC. econs; s; eauto using void_view_join, void_view_bot, void_rmap_expr.
+      all: admit.
+    + admit.
+  - inv STEP. econs; ss.
+    + apply void_rmap_add; ss. econs; eauto using void_view_join, void_view_bot, void_rmap_expr.
+    + inv LC. econs; eauto using void_view_join, void_view_bot, void_rmap_expr.
+    + eauto using void_taint_join, void_taint_bot.
+  - inv STEP. econs; ss.
+    inv LC. econs; s; eauto using void_view_join, void_view_bot, void_rmap_expr.
+  - inv STEP. econs; ss.
+    inv LC. econs; s; eauto using void_view_join, void_view_bot, void_rmap_expr.
+  - inv STEP. econs; ss.
+    inv LC. econs; s; eauto using void_view_join, void_view_bot, void_rmap_expr.
+  - inv STEP. econs; ss.
+    inv LC. econs; s; eauto using void_view_join, void_view_bot, void_rmap_expr.
 Admitted.
 
-Lemma rtc_state_step_certify_inv
-      m1 m2 tid st lc lock
-      (STEPS: rtc (Machine.step ExecUnit.state_step) m1 m2)
-      (NOPROMISE: Machine.no_promise m2)
-      (FIND: IdMap.find tid m1.(Machine.tpool) = Some (st, lc))
-      (CERTIFY: certify tid (ExecUnit.mk st lc m1.(Machine.mem)) lock):
-  lock = Lock.init.
+Lemma void_rtc_aeu_step
+      tid aeu1 aeu2
+      (STEP: rtc (AExecUnit.state_step tid) aeu1 aeu2)
+      (SOUND: void_aeu tid aeu1):
+  void_aeu tid aeu2.
 Proof.
-  destruct lock as [ex release].
-  inv CERTIFY. ss. subst.
+  revert SOUND. induction STEP; ss. i.
+  exploit void_aeu_step; eauto.
+Qed.
+
+Lemma rtc_state_step_certify_bot
+      tid (eu1 eu2:ExecUnit.t (A:=unit))
+      (STEPS: rtc (ExecUnit.state_step tid) eu1 eu2)
+      (NOPROMISE: eu2.(ExecUnit.local).(Local.promises) = bot):
+  certify tid eu1 Lock.init.
+Proof.
+(* TODO:
+ - define eqts
+ - lift_state_step: eu state step -> aeu state step
+ *)
 Admitted.
