src/refinement/PromisingPF_AlgorithmicPF.v
@@ -18,6 +18,7 @@ Require Import Time.
 Require Import Lang.
 Require Import Promising.
 Require Import Algorithmic.
+Require Import Certify.
 Require Import CertifyFacts.
 
 Set Implicit Arguments.
@@ -28,5 +29,12 @@ Theorem promising_pf_to_algorithmic_pf
         (EXEC: Machine.pf_exec p m):
   AMachine.pf_exec p m.
 Proof.
-  inv EXEC. exploit rtc_state_step_certify_bot; eauto.
+  inv EXEC. econs; ss.
+  - instantiate (1 := AMachine.mk m1 (IdMap.map (fun _ => Lock.init) m1.(Machine.tpool))).
+    (* TODO
+     - rtc_state_step_certify_bot : lock.init at last
+     - one step from the end..
+     *)
+    admit.
+  - ss.
 Admitted.
